Mostly-working definition of unary typing

src/Yield.v
@@ -71,7 +71,7 @@ Section parallel.
         | Yield _ s' =>
           fun k' =>
           '(curr', rest') <- choose k' rest;;
-          Tau (par curr' rest' s')
+          Vis (inl1 (Yield _ s')) (fun s' => (par curr' rest' s'))
         end k
       | VisF (inr1 e) k =>
         vis e (fun b => par (fun _ => k b) rest s)
@@ -120,11 +120,10 @@ End parallel.
 
 Variant typing_gen {R} typing (p : perm) (Q : config * R -> Perms) :
   config -> itree (E config) (config * R) -> Prop :=
-| typing_gen_ret r c c' :
+| typing_gen_ret r c :
     pre p c ->
-    p ∈ Q (c', r) ->
-    guar p c c' ->
-    typing_gen typing p Q c (Ret (c', r))
+    (forall c', rely p c c' -> p ∈ Q (c', r)) ->
+    typing_gen typing p Q c (Ret (c, r))
 | typing_gen_tau t c p' :
     pre p c ->
     sep_step p p' -> (* Added since par turns vis into a tau, so the two cases need to be similar... *)
@@ -133,9 +132,17 @@ Variant typing_gen {R} typing (p : perm) (Q : config * R -> Perms) :
 | typing_gen_vis k c c' p' :
     pre p c ->
     guar p c c' ->
+    (* pre p' c' -> *)
     sep_step p p' ->
-    (forall c'', rely p c' c'' -> typing p' Q c (* c'? *) (k c'')) ->
-    typing_gen typing p Q c (vis (Yield _ c') k).
+    (forall c'', rely p c' c'' -> typing p' Q c'' (k c'')) ->
+    typing_gen typing p Q c (Vis (inl1 (Yield _ c')) k)
+(* other events. TODO: generalize E *)
+| typing_gen_e X c p' (e : nondetE X) k :
+    pre p c ->
+    sep_step p p' ->
+    (forall x, typing p' Q c (k x)) ->
+    typing_gen typing p Q c (Vis (inr1 e) k)
+.
 
 Lemma typing_gen_mon {R} : monotone4 (@typing_gen R).
 Proof.
@@ -152,12 +159,25 @@ Lemma typing__lte {R} p Q Q' c (t : itree (E config) (config * R)) :
 Proof.
   revert p Q Q' c t. pcofix CIH. intros p Q Q' c t Htyping Hlte.
   pstep. pinversion Htyping; pclearbot; subst; econstructor; eauto.
-  - apply Hlte; eauto.
+  - intros. apply Hlte; eauto.
   - intros. specialize (H2 _ H3). pclearbot. eauto.
+  - intros. specialize (H1 x). eauto.
 Qed.
 
+(* Lemma typing__lte' p p' Q c (t : itree (E config) (config * unit)) : *)
+(*   typing_ p Q c t -> *)
+(*   p <= p' -> *)
+(*   typing_ p' Q c t. *)
+(* Proof. *)
+(*   revert p p' Q c t. pcofix CIH. intros p p' Q c t Ht Hlte. *)
+(*   pinversion Ht; subst. *)
+(*   - pstep. constructor; auto. *)
+(*     + apply Hlte. *)
+(*     + eapply Perms_upwards_closed; eauto. *)
+(* Qed. *)
+
 Definition typing {R} P Q (t : stateT config (itree (E config)) R) :=
-  forall p c c', p ∈ P -> pre p c -> guar p c c' -> typing_ p Q c (t c').
+  forall p c, p ∈ P -> pre p c -> typing_ p Q c (t c).
 (* also pre p c'? *)
 
 Lemma typing_lte {R} P P' Q Q' (t : stateT config (itree (E config)) R) :
@@ -174,18 +194,20 @@ Lemma typing__bind {R S} p Q1 Q2 c
       (t2 : R -> stateT config (itree (E config)) S)
       r' :
   typing_ p Q1 c t1 ->
-  (forall r p c c', p ∈ Q1 (c', r) ->
-               pre p c ->
-               guar p c c' ->
-               paco4 typing_gen r' p Q2 c (t2 r c')) ->
+  (forall r p c, (forall c', rely p c c' -> p ∈ Q1 (c', r)) ->
+             pre p c ->
+             paco4 typing_gen r' p Q2 c (t2 r c)) ->
   paco4 typing_gen r' p Q2 c (x <- t1;; t2 (snd x) (fst x)).
 Proof.
-  revert p Q1 Q2 c t1 t2. pcofix CIH. intros p Q1 Q2 c t1 t2 Htyping1 Htyping2.
-  pinversion Htyping1; subst.
+  revert p Q1 Q2 c t1 t2. pcofix CIH. intros p Q1 Q2 c t1 t2 Ht1 Ht2.
+  pinversion Ht1; subst.
   - rewritebisim @bind_ret_l. eapply paco4_mon; eauto.
   - rewritebisim @bind_tau. pstep. econstructor; eauto.
   - rewritebisim @bind_vis. pstep. econstructor; eauto. intros.
-    specialize (H2 _ H3). pclearbot. right. eapply CIH; eauto.
+    right. eapply CIH; eauto.
+    specialize (H2 _ H3). pclearbot. apply H2.
+  - rewritebisim @bind_vis. pstep. econstructor; eauto. intros.
+    right. eapply CIH; eauto. apply H1.
 Qed.
 
 Lemma typing_bind {R S} P Q1 Q2
@@ -196,18 +218,8 @@ Lemma typing_bind {R S} P Q1 Q2
   typing P Q2 (bind t1 t2).
 Proof.
   repeat intro. unfold bind. unfold Monad_stateT. red.
-  eapply typing__bind; eauto. intros. eapply H0; eauto.
+  eapply typing__bind; eauto. intros. eapply H0; eauto. apply H3; auto. reflexivity.
 Qed.
-
-Lemma typing__sep_step p p' Q c (t : itree (E config) (config * unit)) :
-  sep_step p p' ->
-  typing_ p' Q c t ->
-  typing_ p Q c t.
-Proof.
-  revert c t. pcofix CIH. intros c t Hstep Ht.
-  punfold Ht. induction Ht.
-  - pstep. constructor; auto.
-Abort.
 
 Lemma typing__par_empty p Q c c' t :
   typing_ p Q c (t c') ->
@@ -222,32 +234,17 @@ Proof.
   - pstep. unfold choose, choose'. rewritebisim @bind_ret_l. econstructor; eauto.
     right. eapply CIH; eauto.
     assert (rely p c'0 c'0) by reflexivity.
-    specialize (H4 _ H3). pclearbot. eauto.
+    specialize (H4 _ H3). pclearbot.
+    apply H4.
+  - pstep. econstructor; eauto. intros. right. apply CIH. apply H3.
 Qed.
 
 Lemma typing_par_empty P Q t :
   typing P Q t ->
   typing P Q (par t []).
 Proof.
-  intros Ht p c c' Hp Hpre Hguar. apply typing__par_empty; auto.
+  intros Ht p c Hp Hpre. apply typing__par_empty; auto.
 Qed.
-
-(* Lemma typing__par_empty' p Q Q' c c' t : *)
-(*   p ∈ Q' tt -> *)
-(*   typing_ p Q c (t c') -> *)
-(*   typing_ p Q c (par t [] c'). *)
-(* Proof. *)
-(*   revert p c c' t. *)
-(*   pcofix CIH. *)
-(*   intros p c c' t Ht. rewrite rewrite_par. unfold par_match. *)
-(*   pinversion Ht; subst; simpl. *)
-(*   - pstep. constructor; auto. destruct r0; auto. *)
-(*   - pstep. econstructor; eauto. *)
-(*   - pstep. unfold choose, choose'. rewritebisim @bind_ret_l. econstructor; eauto. *)
-(*     right. eapply CIH; eauto. *)
-(*     assert (rely p c'0 c'0) by reflexivity. *)
-(*     specialize (H4 _ H3). pclearbot. eauto. *)
-(* Qed. *)
 
 Lemma typing__frame p p' r (Q : config * unit -> Perms) R t c :
   typing_ p Q c t ->
@@ -259,9 +256,9 @@ Proof.
   revert p p' r Q R t c.
   pcofix CIH. intros p p' r' Q R t c Ht Hr Hp' Hpre.
   pinversion Ht; subst.
-  - pstep. constructor; auto.
-    + eapply Perms_upwards_closed; eauto. apply sep_conj_Perms_perm; auto.
-    + apply Hp'. constructor. left. auto.
+  - pstep. constructor; auto. destruct r0. intros.
+    eapply Perms_upwards_closed; eauto. apply sep_conj_Perms_perm; auto.
+    apply H0; auto. apply Hp'; auto.
   - pstep. econstructor; auto.
     + eapply sep_step_lte; eauto. eapply sep_step_sep_conj_l.
       apply Hp' in Hpre. apply Hpre.
@@ -270,7 +267,7 @@ Proof.
       split; [| split]. pinversion H1; auto.
       apply Hp'. apply Hpre.
       apply H0. apply Hp' in Hpre. apply Hpre.
-  - pstep. econstructor; eauto.
+  - pstep. econstructor; auto.
     + apply Hp'. constructor. left. auto.
     + eapply sep_step_lte; eauto. eapply sep_step_sep_conj_l.
       apply Hp' in Hpre. apply Hpre.
@@ -280,9 +277,76 @@ Proof.
       { apply Hp'. auto. }
       specialize (H2 _ H4). pclearbot.
       eapply CIH; eauto. reflexivity.
-      split; [| split]. pinversion H2; auto.
+      split; [| split].
+      * pinversion H2; auto.
+      * pose proof Hpre as Hpre'. apply Hp' in Hpre'. destruct Hpre' as (_ & _ & Hsep).
+        apply Hsep in H0. respects. etransitivity; eauto. apply Hp'. auto. apply Hp'; auto.
+      * apply H1. apply Hp' in Hpre. apply Hpre.
+  - pstep. econstructor; eauto.
+    + eapply sep_step_lte; eauto. eapply sep_step_sep_conj_l.
+      apply Hp' in Hpre. apply Hpre.
+      apply H0.
+    + intros. specialize (H1 x). right. eapply CIH; eauto. reflexivity.
+      split; [| split]. pinversion H1; auto.
+      apply Hp'. auto.
+      apply Hp' in Hpre. apply H0. apply Hpre.
+Qed.
+
+Lemma typing__frame' p p' r (Q R : config * unit -> Perms) t c :
+  typing_ p Q c t ->
+  (forall c', rely r c c' -> r ∈ R (c', tt)) ->
+  r ** p <= p' ->
+  pre p' c ->
+  typing_ p' (fun c => R c * Q c) c t.
+Proof.
+  revert p p' r Q R t c.
+  pcofix CIH. intros p p' r' Q R t c Ht Hr Hp' Hpre.
+  pinversion Ht; subst.
+  - pstep. constructor; auto. destruct r0. intros.
+    eapply Perms_upwards_closed; eauto. apply sep_conj_Perms_perm; auto.
+    + apply Hr; auto. apply Hp'; auto.
+    + apply H0; auto. apply Hp'; auto.
+  - pstep. econstructor; auto.
+    + eapply sep_step_lte; eauto. eapply sep_step_sep_conj_r.
+      apply Hp' in Hpre. destruct Hpre as (_ & _ & Hpre). symmetry in Hpre. apply Hpre.
+      apply H0.
+    + right. eapply CIH; eauto. reflexivity.
+      (* intros. apply Hr. apply Hp'. eapply sep_step_rely; eauto. *)
+
+      split; [| split].
       apply Hp'. apply Hpre.
-      apply H1. apply Hp' in Hpre. apply Hpre.
+      pinversion H1; auto.
+      symmetry. apply H0. apply Hp' in Hpre.
+      destruct Hpre as (_ & _ & Hpre). symmetry in Hpre. apply Hpre.
+  - pstep. econstructor; eauto.
+    + apply Hp'. constructor. right. auto.
+    + eapply sep_step_lte; eauto. eapply sep_step_sep_conj_r; eauto.
+      apply Hp' in Hpre. destruct Hpre as (_ & _ & Hpre). symmetry in Hpre. apply Hpre.
+    + intros. right.
+      assert (rely p c' c'').
+      { apply Hp'. auto. }
+      specialize (H2 _ H4). pclearbot.
+      eapply CIH; eauto. 2: reflexivity.
+
+      intros. apply Hr. etransitivity; eauto.
+      apply Hp' in Hpre. destruct Hpre as (_ & _ & Hsep). transitivity c'.
+      apply Hsep; auto. apply Hp'; auto.
+
+      split; [| split].
+      * pose proof Hpre as Hpre'. apply Hp' in Hpre'. destruct Hpre' as (_ & _ & Hsep).
+        apply Hsep in H0. respects. etransitivity; eauto. apply Hp'. auto. apply Hp'; auto.
+      * pinversion H2; auto.
+      * symmetry. apply H1. apply Hp' in Hpre.
+        destruct Hpre as (_ & _ & Hpre). symmetry in Hpre. apply Hpre.
+  - pstep. econstructor; eauto.
+    + eapply sep_step_lte; eauto. eapply sep_step_sep_conj_r; eauto.
+      apply Hp' in Hpre. destruct Hpre as (_ & _ & Hpre). symmetry in Hpre. apply Hpre.
+    + intros. specialize (H1 x). right. eapply CIH; eauto. reflexivity.
+      split; [| split].
+      apply Hp'. auto.
+      pinversion H1; auto.
+      symmetry. apply Hp' in Hpre. apply H0.
+      destruct Hpre as (_ & _ & Hpre). symmetry in Hpre. apply Hpre.
 Qed.
 
 Lemma typing_frame P P' (Q : config * unit -> Perms) t :
@@ -290,41 +354,101 @@ Lemma typing_frame P P' (Q : config * unit -> Perms) t :
   typing (P * P') (fun r => Q r * P') t.
 Proof.
   repeat intro. destruct H0 as (? & ? & ? & ? & ?).
-  eapply typing__frame; eauto. apply H; auto. apply H4. auto. inversion H4.
-  (* intros Ht p c c' Hp Hpre Hguar. *)
-  revert P P' Q t. pcofix CIH. intros P P' Q t Ht p c c' Hp Hpre Hguar.
-  assert (Hp': p ∈ P).
-  { destruct Hp as (? & ? & ? & ? & ?).
-    eapply Perms_upwards_closed; eauto. etransitivity; eauto.
-    apply lte_l_sep_conj_perm. }
-  specialize (Ht _ _ _ Hp' Hpre Hguar).
-  (* revert Ht Hp Hpre Hguar Hp'. revert P P' Q t p c c'. pcofix CIH. *)
-  (* intros P P' Q t p c c' Ht Hpp' Hpre Hguar Hp. *)
-
-  pinversion Ht; subst.
-  - pstep. constructor; auto. admit.
-  - pstep. econstructor. auto. reflexivity. right.
-    change t0 with ((fun _ => t0) c'). eapply CIH; eauto.
-    repeat intro.
-
+  eapply typing__frame; eauto. apply H; auto. apply H3. auto.
 Qed.
+
+Lemma typing__par p1 p2 p Q1 Q2 c t1 t2 :
+  typing_ p1 Q1 c (t1 c) ->
+  typing_ p2 Q2 c (t2 c) ->
+  p1 ** p2 <= p ->
+  pre p c ->
+  typing_ p (fun c => Q1 c * Q2 c) c (par t1 [t2] c).
+Proof.
+  revert p1 p2 p c t1 t2. pcofix CIH. intros p1 p2 p c t1 t2 Ht1 Ht2 Hlte Hpre.
+  rewrite rewrite_par. unfold par_match. pinversion Ht1; subst; simpl.
+  - destruct r0. pstep. econstructor; eauto. reflexivity. left.
+    eapply paco4_mon_bot; eauto. eapply typing__frame'; eauto.
+    apply typing__par_empty. apply Ht2; auto.
+    intros; eauto.
+  - pstep. econstructor; eauto.
+    2: { right. eapply CIH. apply H3. apply Ht2.
+         reflexivity. split; [| split]; auto.
+         pinversion H3; auto.
+         apply Hlte; auto.
+         apply H1. apply Hlte in Hpre. apply Hpre.
+    }
+    etransitivity; eauto. apply sep_step_lte'; eauto.
+    apply sep_step_sep_conj_l; auto. apply Hlte in Hpre. apply Hpre.
+  - unfold choose, choose', or. rewritebisim @bind_vis. simpl.
+    pstep. econstructor; eauto. reflexivity.
+    intros []; left; rewritebisim @bind_ret_l.
+    + pstep. econstructor; auto.
+      * apply Hlte. constructor 1; auto.
+      * eapply sep_step_lte; eauto. apply sep_step_sep_conj_l; eauto.
+        apply Hlte in Hpre. apply Hpre.
+      * intros. right. eapply CIH; eauto.
+        -- assert (Hrely : rely p1 c' c''). apply Hlte; auto.
+           specialize (H4 _ Hrely). pclearbot. eauto.
+        -- admit.
+        -- reflexivity.
+        -- split; [| split].
+           ++ apply Hlte in H3. destruct H3. specialize (H4 _ H3).
+              pclearbot. pinversion H4; auto.
+           ++ respects; auto. apply Hlte; eauto.
+              apply Hlte in Hpre. pose proof Hpre as (_ & _ & Hsep).
+              respects; eauto. apply Hsep; eauto. apply Hpre.
+           ++ apply H2; auto. apply Hlte in Hpre. apply Hpre.
+    + admit.
+  - pstep. econstructor; auto.
+    2: { intros. specialize (H3 x). right. eapply CIH. apply H3. eauto. reflexivity.
+         split; [| split].
+         - pinversion H3; auto.
+         - apply Hlte; auto.
+         - apply H1. apply Hlte in Hpre. apply Hpre. }
+    eapply sep_step_lte; eauto. apply sep_step_sep_conj_l; auto.
+    apply Hlte in Hpre. apply Hpre.
+Admitted.
 
 Lemma typing_par P1 P2 (Q1 Q2 : config * unit -> Perms) t1 t2 :
   typing P1 Q1 t1 ->
   typing P2 Q2 t2 ->
-  typing (P1 * P2) (fun '(c, _) => Q1 (c, tt) * Q2 (c, tt)) (par t1 [t2]).
+  typing (P1 * P2) (fun c => Q1 c * Q2 c) (par t1 [t2]).
 Proof.
-  revert t1 t2 P1 P2 Q1 Q2.
-  pcofix CIH. intros t1 t2 P1 P2 Q1 Q2.
-  intros Ht1 Ht2 p c c' (p1 & p2 & Hp1 & Hp2 & Hlte) Hpre Hguar.
-  rewrite rewrite_par. unfold par_match.
-  assert (Hp1': p ∈ P1) by admit.
-  specialize (Ht1 _ _ _ Hp1' Hpre Hguar). pinversion Ht1; subst; simpl.
-  - destruct r0. pstep. econstructor; eauto. reflexivity. left.
-    (* How do we push through the stronger post-condition here? p can change arbitrarily in the typing computation for t2, so why does this hold? *)
-    eapply typing_par_empty in Ht2.
-    red in Ht2.
-    eapply paco4_mon_bot. apply Ht2; eauto. admit.
-    intros. eauto.
-  -
+
+  repeat intro. destruct H1 as (? & ? & ? & ? & ?).
+  eapply typing__par; eauto. unfold typing in *.
+  apply H; auto. apply H4; auto.
+  apply H0; auto. apply H4; auto.
+
+  (* (* revert t1 t2 P1 P2 Q1 Q2. *) *)
+  (* intros Ht1 Ht2 p c (p1 & p2 & Hp1 & Hp2 & Hlte) Hpre. *)
+  (* assert (Hpre1 : pre p1 c). { apply Hlte; auto. } *)
+  (* assert (Hpre2 : pre p2 c). { apply Hlte; auto. } *)
+  (* specialize (Ht1 _ _ Hp1 Hpre1). *)
+  (* specialize (Ht2 _ _ Hp2 Hpre2). *)
+  (* revert Ht1 Ht2 Hp1 Hp2 Hlte Hpre Hpre1 Hpre2. revert t1 t2 c p1 p2 p (* P1 P2 Q1 Q2 *). *)
+  (* (* pcofix CIH. *) intros t1 t2 c p1 p2 p (* P1 P2 Q1 Q2 *). *)
+  (* intros Ht1 Ht2 Hp1 Hp2 Hlte Hpre Hpre1 Hpre2. *)
+  (* rewrite rewrite_par. unfold par_match. pinversion Ht1; subst; simpl. *)
+  (* - destruct r0. pstep. econstructor; eauto. reflexivity. left. *)
+  (*   eapply paco4_mon_bot; eauto. eapply typing__frame'; eauto. *)
+  (*   apply typing__par_empty. apply Ht2; auto. *)
+  (*   intros; eauto. *)
+  (* - pstep. econstructor; eauto. *)
+  (*   2: { right. eapply CIH. apply H3. apply Ht2. all: auto. *)
+  (*        admit. (* we need typing_ version... *) *)
+  (*        reflexivity. split; [| split]; auto. *)
+  (*        pinversion H3; auto. *)
+  (*        apply H1. apply Hlte in Hpre. apply Hpre. *)
+  (*        pinversion H3; auto. *)
+  (*   } *)
+  (*   etransitivity; eauto. apply sep_step_lte'; eauto. *)
+  (*   apply sep_step_sep_conj_l; auto. apply Hlte in Hpre. apply Hpre. *)
+  (* - unfold choose, choose', or. rewritebisim @bind_vis. simpl. *)
+  (*   pstep. econstructor; eauto. reflexivity. *)
+  (* - eapply typing_par_empty in Ht2. *)
+  (*   red in Ht2. *)
+  (*   eapply paco4_mon_bot. apply Ht2; eauto. admi.t *)
+  (*   intros. eauto. *)
+  (* - *)
 Qed.
